HeapLang/WeakestPrecondition.thy
@@ -1,0 +1,12 @@
+theory WeakestPrecondition
+imports "../IrisCore/BaseLogicShallow" "../IrisCore/AuthHeap" HeapLang State
+begin
+
+subsection \<open>Weakest Preconditions\<close>
+context fixes red :: "expr \<Rightarrow> state \<Rightarrow> ('a::ucamera) iprop"
+  and step :: "expr \<Rightarrow> state \<Rightarrow> expr \<Rightarrow> state \<Rightarrow> expr list \<Rightarrow> 'a iprop"
+begin
+fun wp :: "expr \<Rightarrow> (val \<Rightarrow> 'a iprop) \<Rightarrow> 'a iprop" where
+  "wp e \<Phi> = (case to_val e of Some v \<Rightarrow> \<Phi> v 
+    | None \<Rightarrow> \<forall>\<^sub>u(\<lambda>\<sigma>. red e \<sigma> \<and>\<^sub>u \<triangleright>(\<forall>\<^sub>u(\<lambda>(e2,\<sigma>2). (step e \<sigma> e2 \<sigma>2 []) -\<^emph> wp e2 \<Phi>))))"
+end
